

OPT 570 Practice Exam 1

Problem 1

a. $\begin{pmatrix} 0 \\ 0 \\ 1 \end{pmatrix}$

b. $(0 \ 1 \ 0)$

c. $\begin{pmatrix} 0 & 0 & 0 \\ 0 & 0 & 0 \\ 0 & 1 & 0 \end{pmatrix} = \begin{pmatrix} 0 \\ 0 \\ 1 \end{pmatrix} (0 \ 1 \ 0)$

d. $\begin{pmatrix} 1/2 \\ -1/\sqrt{2} \\ 1/2 \end{pmatrix}$

e. $-1/\sqrt{2} = (0 \ 1 \ 0) \begin{pmatrix} 1/2 \\ -1/\sqrt{2} \\ 1/2 \end{pmatrix}$

f. $1 = \begin{pmatrix} 1 & 0 & 0 \\ 0 & 1 & 0 \\ 0 & 0 & 1 \end{pmatrix}$ closure
rel.

g. $\begin{pmatrix} -\hbar\omega & 0 & 0 \\ 0 & 0 & 0 \\ 0 & 0 & \hbar\omega \end{pmatrix}$

h. $\begin{pmatrix} e^{i\omega t} & 0 & 0 \\ 0 & 1 & 0 \\ 0 & 0 & e^{-i\omega t} \end{pmatrix}$

i. $\begin{pmatrix} e^{-i\omega t} & 0 & 0 \\ 0 & 1 & 0 \\ 0 & 0 & e^{i\omega t} \end{pmatrix} \begin{pmatrix} 1/2 \\ -1/\sqrt{2} \\ 1/2 \end{pmatrix} = \begin{pmatrix} \frac{1}{2} e^{-i\omega t} \\ -1/\sqrt{2} \\ \frac{1}{2} e^{i\omega t} \end{pmatrix}$

j. $\hat{P}_S = |a_3\rangle\langle a_3|$ $\hat{P}_H = \underbrace{\hat{U}^\dagger}_i |a_3\rangle\langle a_3| \underbrace{\hat{U}}_{\text{conj of } i} = \begin{pmatrix} \frac{1}{2} e^{-i\omega t} \\ -1/\sqrt{2} \\ \frac{1}{2} e^{i\omega t} \end{pmatrix} \begin{pmatrix} \frac{1}{2} e^{i\omega t} & \frac{1}{\sqrt{2}} & \frac{1}{2} e^{-i\omega t} \end{pmatrix}$

$= \begin{pmatrix} \frac{1}{4} & -\frac{1}{2\sqrt{2}} e^{-i\omega t} & \frac{1}{4} e^{-2i\omega t} \\ -\frac{1}{2\sqrt{2}} e^{+i\omega t} & \frac{1}{2} & -\frac{1}{2\sqrt{2}} e^{-i\omega t} \\ \frac{1}{4} e^{2i\omega t} & -\frac{1}{2\sqrt{2}} e^{i\omega t} & \frac{1}{4} \end{pmatrix}$

Hermitian ✓
Trace = 1 ✓

Problem 2

$\text{FT}[\psi(x-x_0)] = \langle p | \hat{S}(x_0) | \psi \rangle =$
 $= e^{-ix_0 p/\hbar} \langle p | \psi \rangle =$
 $= e^{-ix_0 p/\hbar} \tilde{\psi}(p)$

Problem 3

a.

$e^{+ip_0 \hat{x}/\hbar}$	- translates in momentum space by p_0
$e^{-ip_0 \hat{x}/\hbar}$	- ——— ——— by $-p_0$
$e^{-ix_0 \hat{p}/\hbar}$	- ——— ——— in position space by x_0
$e^{ix_0 \hat{p}/\hbar}$	- ——— ——— by $-x_0$

Overall, the operator brings state back to initial position

$$\hat{A} = 1^n = 1$$

b. Projector onto the $x_0 - \sigma$ to $x_0 + \sigma$ part of the position axis

$$\underline{c} \quad \hat{C} = \int_{-\infty}^{+\infty} dx' |x'\rangle F(x') \langle x'|$$

in pos: $\langle x | \hat{C} | \rangle = \int_{-\infty}^{+\infty} dx' \underbrace{\langle x | x' \rangle}_{\delta(x-x')} F(x') \langle x' | =$

$$= F(x) - x$$

impos. representation, \hat{C} multiplies state by $F(x)$

To be projector, $\hat{C}^2 = \hat{C}$

$$\hat{C}^2 = \int_{-\infty}^{+\infty} \int_{-\infty}^{+\infty} dx' dx'' \underbrace{|x' X x'| F X x'| x'' X x''| F X x''}_{\delta(x' - x'')} =$$

$$= \int_{-\infty}^{+\infty} dx' \langle x' | X | x' \rangle \langle x' | F | x' \rangle =$$

$$= \int_{-\infty}^{+\infty} |\langle x' | F \rangle|^2 |x' \rangle \langle x'| dx'$$

$$\hat{C} = \int_{-\infty}^{\infty} |\langle x' | F \rangle|^2 |x' \rangle \langle x'| dx'$$

$$\hat{C}^2 = \hat{C} \text{ only if } F(x)^2 = F(x) \text{ for all } x$$

So $F(x) = \begin{cases} 0 \\ 1 \end{cases}$ or piece wise

Problem 4 $\hat{B} = \sum_{m=-2}^2 |m\rangle \langle -m \times m|$

a $\langle \psi | \hat{N} | \psi \rangle = ?$
 $\hat{N} | \psi \rangle = \begin{pmatrix} 2 \cdot \frac{1}{2} \\ 1 \cdot \frac{1}{\sqrt{2}} \\ 0 \cdot \frac{1}{2} \\ 0 \\ 0 \end{pmatrix} = \begin{pmatrix} 1 \\ 1/\sqrt{2} \\ 0 \\ 0 \\ 0 \end{pmatrix}$

$\langle \psi | \hat{N} | \psi \rangle = \left(\frac{1}{2} \quad \frac{1}{\sqrt{2}} \quad \frac{1}{2} \quad 0 \quad 0 \right) \begin{pmatrix} 1 \\ 1/\sqrt{2} \\ 0 \\ 0 \\ 0 \end{pmatrix} = \frac{1}{2} + \frac{1}{2} = \boxed{1}$

b $\hat{B} \rightarrow \begin{pmatrix} 0 & 0 & 0 & 0 & 2 \\ 0 & 0 & 0 & 1 & 0 \\ 0 & 0 & 0 & 0 & 0 \\ 0 & 1 & 0 & 0 & 0 \\ 2 & 0 & 0 & 0 & 0 \end{pmatrix} \Rightarrow \begin{array}{l} B \text{ is Hermitian} \\ B \text{ is not unitary} \end{array}$

c $\text{Tr } \hat{B} = 0$

d $|\varphi\rangle \equiv c \hat{B} |\psi\rangle$ - normalized

$|\varphi\rangle \rightarrow c \cdot \begin{pmatrix} 0 & 0 & 0 & 0 & 2 \\ 0 & 0 & 0 & 1 & 0 \\ 0 & 0 & 0 & 0 & 0 \\ 0 & 1 & 0 & 0 & 0 \\ 2 & 0 & 0 & 0 & 0 \end{pmatrix} \begin{pmatrix} 1 \\ 1/\sqrt{2} \\ 0 \\ 1/\sqrt{2} \\ 0 \end{pmatrix} = c \cdot \begin{pmatrix} 0 \\ 0 \\ 0 \\ 1/\sqrt{2} \\ 1 \end{pmatrix}$

$\langle \varphi | \varphi \rangle = 1 \Rightarrow c^2 \cdot \left(\frac{1}{2} + 1 \right) = 1 \Rightarrow \boxed{c = \sqrt{\frac{2}{3}}}$

$|\varphi\rangle \rightarrow \begin{pmatrix} 0 \\ 0 \\ 0 \\ \sqrt{1/3} \\ \sqrt{2/3} \end{pmatrix} \quad \hat{N} |\varphi\rangle \rightarrow \begin{pmatrix} 0 \\ 0 \\ 0 \\ -\sqrt{1/3} \\ -2\sqrt{2/3} \end{pmatrix}$

$\langle \varphi | \hat{N} | \varphi \rangle = -\frac{1}{3} - \frac{4}{3} = -\frac{5}{3}$

$$c) \quad |\beta_1\rangle \equiv \nu|m=-1\rangle + \nu|m=1\rangle \quad \hat{B}|\beta_1\rangle = |\beta_1\rangle$$

$$\hat{B}|\beta_1\rangle = \nu|-1\rangle + \nu|1\rangle \Rightarrow |\beta_1\rangle = \frac{1}{\sqrt{2}}(|-1\rangle + |1\rangle)$$

$$f) \quad \underline{\lambda = 2} \Rightarrow |\beta_2\rangle = \frac{1}{\sqrt{2}}(|2\rangle + |-2\rangle)$$

$$\underline{\lambda = -1} \Rightarrow |\beta_{-1}\rangle = \frac{1}{\sqrt{2}}(|1\rangle - |-1\rangle)$$

$$\underline{\lambda = -2} \Rightarrow |\beta_{-2}\rangle = \frac{1}{\sqrt{2}}(|2\rangle - |-2\rangle)$$

$$\underline{\lambda = 0} \Rightarrow |\beta_0\rangle = |0\rangle$$

$$g) \quad \text{From above: } |2\rangle = \frac{1}{\sqrt{2}}(|\beta_2\rangle + |\beta_{-2}\rangle) \\ |1\rangle = \frac{1}{\sqrt{2}}(|\beta_1\rangle + |\beta_{-1}\rangle)$$

$$\Rightarrow |\psi\rangle = \frac{1}{2\sqrt{2}}|\beta_2\rangle + \frac{1}{2\sqrt{2}}|\beta_{-2}\rangle + \frac{1}{2}|\beta_1\rangle + \frac{1}{2}|\beta_{-1}\rangle + \frac{1}{2}|\beta_0\rangle$$

$$h) \quad \langle 1|e^{i\theta\hat{B}}|1\rangle \quad e^{i\theta\hat{B}} \cdot \frac{1}{\sqrt{2}}(|\beta_1\rangle + |\beta_{-1}\rangle) \quad e^{i\theta\hat{B}}_{\beta_1} = \begin{pmatrix} e^{2i\theta} & 0 & 0 \\ 0 & e^{i\theta} & 0 \\ 0 & 0 & e^{-i\theta} \end{pmatrix}$$

$$\Rightarrow e^{i\theta\hat{B}}|1\rangle = \frac{1}{\sqrt{2}}(e^{i\theta}|\beta_1\rangle + e^{-i\theta}|\beta_{-1}\rangle)$$

$$\langle 1|e^{i\theta\hat{B}}|1\rangle = \frac{1}{2}(e^{i\theta} + e^{-i\theta}) = \cos\theta$$

Problem 5

$$[a] \quad \hat{H} \rightarrow \frac{\hbar\omega}{2} \begin{pmatrix} 1 & 0 & 0 \\ 0 & 3 & -i\sqrt{3} \\ 0 & +i\sqrt{3} & 5 \end{pmatrix} \Rightarrow \frac{\hbar\omega}{2} \text{ and } \underline{\begin{pmatrix} 1 \\ 0 \\ 0 \end{pmatrix}}$$

For other two $\begin{vmatrix} 3-\lambda & -i\sqrt{3} \\ i\sqrt{3} & 5-\lambda \end{vmatrix} = 0 \quad (3-\lambda)(5-\lambda) - 3 = 0$
 $\lambda^2 - 8\lambda + 12 = 0 \quad (\lambda-6)(\lambda-2) = 0$

$$\underline{\lambda=2} \quad \begin{pmatrix} 3 & -i\sqrt{3} \\ i\sqrt{3} & 5 \end{pmatrix} \begin{pmatrix} v_1 \\ v_2 \end{pmatrix} = \begin{pmatrix} 2v_1 \\ 2v_2 \end{pmatrix} \Rightarrow -i\sqrt{3}v_2 = v_1$$

$$\Rightarrow \begin{pmatrix} 1 \\ -\frac{i}{\sqrt{3}} \end{pmatrix} \Rightarrow \frac{1}{\sqrt{1+\frac{1}{3}}} \begin{pmatrix} 1 \\ -\frac{i}{\sqrt{3}} \end{pmatrix} = \underline{\begin{pmatrix} \sqrt{3}/2 \\ -i/2 \end{pmatrix}}$$

$$\underline{\lambda=6} \quad \begin{pmatrix} 3 & -i\sqrt{3} \\ i\sqrt{3} & 5 \end{pmatrix} \begin{pmatrix} v_1 \\ v_2 \end{pmatrix} = \begin{pmatrix} 6v_1 \\ 6v_2 \end{pmatrix} \Rightarrow -i\sqrt{3}v_2 = 3v_1$$

$$\Rightarrow \begin{pmatrix} 1 \\ i\sqrt{3} \end{pmatrix} \Rightarrow \frac{1}{\sqrt{1+3}} \begin{pmatrix} 1 \\ i\sqrt{3} \end{pmatrix} = \underline{\begin{pmatrix} 1/2 \\ i\sqrt{3}/2 \end{pmatrix}}$$

$$\frac{\hbar\omega}{2} \begin{pmatrix} 1 \\ 0 \\ 0 \end{pmatrix}$$

$$\frac{\hbar\omega}{2} \begin{pmatrix} 0 \\ \sqrt{3}/2 \\ -i/2 \end{pmatrix}$$

$$\frac{3\hbar\omega}{2} \begin{pmatrix} 0 \\ 1/2 \\ i\sqrt{3}/2 \end{pmatrix}$$

$$[b] \quad \hat{U}(t,0) = e^{-i\hat{H}t/\hbar}$$

$$\hat{U}_{\{u\}} = \begin{pmatrix} e^{-i\omega t/2} & 0 & 0 \\ 0 & e^{-i\omega t} & 0 \\ 0 & 0 & e^{-i3\omega t} \end{pmatrix} \quad M = \begin{pmatrix} 1 & 0 & 0 \\ 0 & \sqrt{3}/2 & 1/2 \\ 0 & -i/2 & i\sqrt{3}/2 \end{pmatrix}$$

$$\hat{U}_{\{u\}} = M^\dagger \hat{U}_{\{u\}} M \Rightarrow \hat{U}_{\{u\}} = M \hat{U}_{\{u\}} M^\dagger =$$

$$= \begin{pmatrix} 1 & 0 & 0 \\ 0 & \sqrt{3}/2 & 1/2 \\ 0 & -i/2 & i\sqrt{3}/2 \end{pmatrix} \begin{pmatrix} e^{-i\omega t/2} & 0 & 0 \\ 0 & e^{-i\omega t} & 0 \\ 0 & 0 & e^{-i3\omega t} \end{pmatrix} \begin{pmatrix} 1 & 0 & 0 \\ 0 & \sqrt{3}/2 & i/2 \\ 0 & 1/2 & -i\sqrt{3}/2 \end{pmatrix} =$$

$$= \begin{pmatrix} e^{-i\omega t/2} & 0 \\ 0 & \frac{3}{4}e^{-i\omega t} + \frac{1}{4}e^{-i3\omega t} & i\frac{\sqrt{3}}{4}e^{-i\omega t} - i\frac{\sqrt{3}}{4}e^{-i3\omega t} \\ 0 & -i\frac{\sqrt{3}}{4}e^{-i\omega t} + i\frac{\sqrt{3}}{4}e^{-i3\omega t} & \frac{1}{4}e^{-i\omega t} + \frac{3}{4}e^{-i3\omega t} \end{pmatrix}$$

c) $|\Psi(0)\rangle = |\Phi_2\rangle$

$$\Rightarrow |\Psi(t)\rangle = \hat{U}_{\zeta\Phi\zeta} \cdot \begin{pmatrix} 0 \\ 1 \\ 0 \end{pmatrix} = \begin{pmatrix} 0 \\ \frac{3}{4}e^{i\omega t} + \frac{1}{4}e^{-i3\omega t} \\ i\frac{\sqrt{3}}{4}e^{-i\omega t} - i\frac{\sqrt{3}}{4}e^{-i3\omega t} \end{pmatrix}$$

d) $P_3(t) = |\langle \Phi_3 | \Psi(t) \rangle|^2 =$

$$= \frac{3}{16} \left(e^{-i\omega t} - e^{-i3\omega t} \right)^2 = \frac{3}{16} \underbrace{(e^{-i2\omega t})^2}_1 \underbrace{(e^{i\omega t} - e^{-i\omega t})^2}_{2 \cdot \sin^2 \omega t}$$

$$= \frac{3}{16} \cdot 4 \cdot \sin^2 \omega t = \boxed{\frac{3}{4} \sin^2 \omega t}$$

